exec-defthms.lisp
@@ -16,14 +16,18 @@
     (implies (env/validp e)
              (env/validp (env/step e))))
 
-;; The proof checking takes 12000+ seconds.
-(defthm env/exec-hacky-io-pc-validp
-    (implies (env/validp e)
-             (integerp (env/pc (env/exec-hacky e n)))))
+;; ;; The proof checking takes 12000+ seconds.
+;; (defthm env/exec-hacky-io-pc-validp
+;;     (implies (env/validp e)
+;;              (integerp (env/pc (env/exec-hacky e n))))
+;;   :hints (("Goal" :in-theory (disable stack/pop
+;;                                       stack/push))))
 
 ;; (defthm env/exec-hacky-io-validp
 ;;     (implies (env/validp e)
-;;              (env/validp (env/exec-hacky e n))))
+;;              (env/validp (env/exec-hacky e n)))
+;;   :hints (("Goal" :in-theory (disable stack/pop
+;;                                       stack/push))))
 
 ;; (defthm env/exec-valid-io
 ;;     (implies (env/validp e)
