stack-defthms.lisp
@@ -2,18 +2,42 @@
 
 (include-book "stack")
 
+(defthm stack/empty-validp
+  (stack/validp (list 'stack-bottom)))
+
 (defthm stack/push-io-validp
     (implies (stack/validp s)
-             (stack/validp (stack/push s v))))
+             (stack/validp (stack/push s v)))
+  :hints (("Goal"
+           :in-theory (enable stack/validp stack/push))))
 
 (defthm stack/pop-io-validp
     (implies (stack/validp s)
-             (stack/validp (stack/pop s))))
+             (stack/validp (stack/pop s)))
+  :hints (("Goal"
+           :in-theory (enable stack/validp stack/pop))))
 
 (defthm stack/popn-io-validp
     (implies (stack/validp s)
-             (stack/validp (stack/popn s n))))
+             (stack/validp (stack/popn s n)))
+  :hints (("Goal"
+           :in-theory (enable stack/validp))))
 
 (defthm stack/validp-implies-consp
     (implies (stack/validp s)
-             (consp s)))
+             (consp s))
+  :hints (("Goal"
+           :in-theory (enable stack/validp))))
+
+(defthm stack/push-then-pop-unchanged
+    (implies (evm-w256p n)
+             (equal (stack/pop (stack/push stack n))
+                    stack))
+  :hints (("Goal"
+           :in-theory (enable stack/push stack/pop))))
+
+(defthm stack/top-evm-w256p
+    (implies (stack/validp s)
+             (evm-w256p (stack/top s)))
+  :hints (("Goal"
+           :in-theory (enable stack/validp stack/top))))
